theories/program_logic/itreewp.v
@@ -9,362 +9,352 @@ Set Default Proof Using "Type".
 Section itreewp.
   Context `{!invGS Σ}. 
 
-(* Curry the value R so it can be changed by the dependent pattern match on c *)
-Definition command_predicate {V R} (c: envE V R) (σ σ': gmap loc V): R -> Prop.
-refine (
-  match c with
-  | GetE l           => λ v, σ !! l = Some v /\ σ' = σ 
-  | PutE l v'        => λ _, is_Some (σ !! l) /\ σ' = <[l := v']> σ
-  | AllocE v'        => λ l, l = fresh_loc σ /\ σ' = <[l := v']> σ
-  | FreeE l          => λ _, is_Some (σ !! l) /\ σ' = delete l σ
-  | CmpXchgE l v1 v2 => λ '(vret, upd), if upd then σ !! l = Some v1 /\ vret = v1 /\ σ' = <[l := v2]> σ  
-                                   else ∃x, σ !! l = Some x /\ vret = x /\ σ = σ' /\ x ≠ v1
-  | FailE            => λ v, False
-  end
-).
-Defined.
+  (* Curry the value R so it can be changed by the dependent pattern match on c *)
+  Definition command_predicate {V R} (c: envE V R) (σ σ': gmap loc V): R -> Prop :=
+    match c with
+    | GetE l           => λ v, σ !! l = Some v /\ σ' = σ 
+    | PutE l v'        => λ _, is_Some (σ !! l) /\ σ' = <[l := v']> σ
+    | AllocE v'        => λ l, l = fresh_loc σ /\ σ' = <[l := v']> σ
+    | FreeE l          => λ _, is_Some (σ !! l) /\ σ' = delete l σ
+    | CmpXchgE l v1 v2 => λ '(vret, upd), if upd then σ !! l = Some v1 /\ vret = v1 /\ σ' = <[l := v2]> σ  
+                                          else ∃x, σ !! l = Some x /\ vret = x /\ σ = σ' /\ x ≠ v1
+    | FailE            => λ v, False
+    end.
 
-Definition wp_pre {V} (SI: gmap loc V -> iProp Σ)
-     (go: discrete_funO (λ R, coPset -d> expr V R -d> (R -d> iPropO Σ) -d> iPropO Σ)):
-     discrete_funO (λ R, coPset -d> expr V R -d> (R -d> iPropO Σ) -d> iPropO Σ).
-refine(λ R E e Φ,
+  Definition wp_pre {V} (SI: gmap loc V -> iProp Σ)
+    (go: discrete_funO (λ R, coPset -d> expr V R -d> (R -d> iPropO Σ) -d> iPropO Σ)):
+    discrete_funO (λ R, coPset -d> expr V R -d> (R -d> iPropO Σ) -d> iPropO Σ) :=
+      λ R E e Φ,
         match e with
         |Answer x  => |={E}=> Φ x 
         |Think e'  => |={E, ∅}=> ▷ |={∅, E}=> go R E e' Φ
         |Fork e' k => |={E, ∅}=> ▷ |={∅, E}=> (go R E k Φ ∗ go unit ⊤ e' (λ _, True))
-        (* make wp less determinstic  *)
-        (* |Vis c k   => ∀σ, SI σ ==∗ ▷ |==> (∃σ' v, ⌜command_predicate c σ σ' v⌝) ∗
-            ∀ σ' v, ⌜command_predicate c σ σ' v⌝ -∗ SI σ' ∗ (go R (k v)) Φ *)
         |Vis c k   => ∀σ, SI σ ={E, ∅}=∗ ▷ |={∅, E}=> ∃σ' v, ⌜command_predicate c σ σ' v⌝ ∗ SI σ' ∗ (go R E (k v)) Φ
-        end
-)%I.
-Defined.
+        end%I.
 
-Instance wp_pre_contractive {A SI}: Contractive (@wp_pre A SI).
-Proof.
-  rewrite /wp_pre => n wp wp' Hwp R E e1 Φ.
-  repeat (f_contractive || f_equiv); apply Hwp.
-Qed.
-
-Definition wp' {V} (SI: gmap nat V -> iProp Σ)
-              : ∀R, coPset -> expr V R -> (R -> iProp Σ) ->iProp Σ :=
-    fixpoint (wp_pre SI ).
-
-Definition wp {V R} (SI: gmap nat V -> iProp Σ) (E: coPset) (e: expr V R) (Φ: R -> iProp Σ): iProp Σ := 
-    wp' SI R E e Φ.
-
-Definition wp_thread {V R} (SI: gmap nat V -> iProp Σ) (t: thread V R) 
-: (R -> iProp Σ) -> iProp Σ.
-refine (
-  match t with
-  | Main e => wp SI ⊤ e
-  | Forked e => λ _,  wp SI ⊤ e (λ _, True)
-  end
-)%I.
-Defined.
-
-Lemma wp'_unfold {V R} (SI: gmap nat V -> iProp Σ) (E: coPset) (e: expr V R)  (Φ: R -> iProp Σ)
-  : wp' SI R E e Φ  ≡  wp_pre SI (wp' SI) R E e Φ.
-Proof.
-  apply (fixpoint_unfold (wp_pre SI)).
-Qed.
-
-Lemma wp_unfold {V R} (SI: gmap nat V -> iProp Σ) (E: coPset) (e: expr V R)  (Φ: R -> iProp Σ)
-  : wp SI E e Φ  ≡  wp_pre SI (wp' SI) R E e Φ.
-Proof.
-  apply (fixpoint_unfold (wp_pre SI)).
-Qed.
-
-Lemma wp_return {V R: Type} (SI: gmap nat V -> iProp Σ) (E: coPset)
-   (x: R) (Φ: R -> iProp Σ): Φ x -∗ wp SI E (mret x) Φ.
-Proof.
-  iIntros"H".
-  by rewrite wp_unfold.
-Qed.
-
-Lemma wp_think {V R: Type} (SI: gmap nat V -> iProp Σ) (E: coPset)
-   (e: expr V R) (Φ: R -> iProp Σ): ▷ wp SI E e Φ -∗ wp SI E (Think e) Φ.
-Proof.
-  iIntros "Hwp".
-  iEval (rewrite wp_unfold).
-  unfold wp_pre.
-  iApply fupd_mask_intro; first set_solver.
-  iIntros "H".
-  iNext. iMod "H". iModIntro.
-  done.
-Qed.
-
-Lemma wp_bind {V R B: Type} (SI: gmap nat V -> iProp Σ) (E: coPset)
-  (f: R -> expr V B) (Φ: B -> iProp Σ) (e: expr V R):
-  wp SI E e (λ x, wp SI E (f x) Φ) -∗ wp SI E (e ≫= f) Φ.
-Proof.
-  unfold mbind, itree_bind.
-  iIntros "H". iLöb as "IH" forall (e).
-  iEval (rewrite wp_unfold).
-  unfold wp_pre.
-  destruct e; simpl.
-  - do 2 (rewrite wp_unfold /=). unfold wp_pre.
-    by destruct (f r); iMod "H".
-  - iEval (rewrite wp_unfold /=) in "H".
-    iMod "H". iIntros "!> !>". iApply "IH". done.
-  - iEval (rewrite wp_unfold /=) in "H".
-    iMod "H". iIntros "!> !>". iMod "H" as "(H & $)".
-    iApply "IH". done.
-  - iIntros (σ)  "HSi".
-    iEval (rewrite wp_unfold /=) in "H".
-    iMod ("H" $! σ with "HSi") as "H". iModIntro.
-    iNext.
-    iMod ("H") as (σ' v) "H". iModIntro.
-    iExists σ', v.
-    iDestruct "H" as "($ & $ & Hwp)".
-    iApply "IH". done.
-Qed.
-
-Lemma wp_vup {V R: Type} (SI: gmap nat V -> iProp Σ) (E: coPset)
-  (e: expr V R) (Φ: R -> iProp Σ)
-  : (|={E}=> wp SI E e (λ v, |={E}=> Φ v)) ⊢ wp SI E e Φ.
-Proof.
-  iLöb as "IH" forall (e).
-  iIntros "Hwp".
-  rewrite wp_unfold. rewrite wp_unfold.
-  unfold wp_pre.
-  destruct e; simpl.
-  - repeat (iMod "Hwp"). done.
-  - iMod "Hwp". 
-    iMod "Hwp". iModIntro.
-    iNext. 
-    iMod "Hwp". iModIntro.
-    iApply "IH". done.
-  - repeat (iMod "Hwp").
-    iModIntro. iNext.
-    iMod "Hwp" as "(Hwp & $)".
-    iApply "IH". done.
-  - iIntros (σ) "HSi".
-    iMod "Hwp".
-    iDestruct ("Hwp" with "HSi" ) as "Hwp".
-    iMod "Hwp". iModIntro. iNext.
-    iMod "Hwp". iModIntro.
-    iDestruct ("Hwp") as (σ' v) "(Hcmd & HSi & Hwp)".
-    iExists σ', v. iFrame.
-    iApply "IH". done.
-Qed.
-
-Inductive atomic {V R: Type}: expr V R -> Prop :=
-|answer_atomic:  ∀ x, atomic (Answer x)
-|think_atomic:  ∀ x, atomic (Think (Answer x))
-|vis_atomic: ∀c, atomic (Vis c Answer).
-
-Lemma wp_atomic {V R: Type} (SI: gmap nat V -> iProp Σ) (E1 E2: coPset)
-  (e: expr V R) (Φ: R -> iProp Σ)
-  (a: atomic e)
-  : (|={E1, E2}=> wp SI E2 e (λ v, |={E2, E1}=> Φ v)) ⊢ wp SI E1 e Φ.
-Proof.
-  iIntros "Hwp".
-  rewrite wp_unfold. 
-  rewrite wp_unfold. 
-  destruct a; simpl.
-  - iMod "Hwp". iMod "Hwp". iMod "Hwp".
-    done.
-  - iMod "Hwp". iMod "Hwp". iModIntro.
-    iNext. iMod "Hwp". 
-    rewrite wp'_unfold. rewrite wp'_unfold. simpl.
-    iMod "Hwp".  iMod "Hwp". done.
-  - iIntros (σ) "HSi".
-    iMod "Hwp". iDestruct ("Hwp" with "HSi") as "Hwp".
-    iMod "Hwp". iModIntro. iNext. iMod "Hwp".
-    iDestruct ("Hwp") as (σ' v) "(Hcmd & HSi & Hwp)".
-    iExists σ', v. iFrame.
-    rewrite wp'_unfold. rewrite wp'_unfold. simpl.
-    iMod "Hwp". iMod "Hwp".
-    done.
-Qed.
-
-Lemma wp_strong_mono_fupd {V R: Type} (SI: gmap nat V -> iProp Σ) (E1 E2: coPset)
-  (e: expr V R) (Φ Ψ: R -> iProp Σ)
-  : E1 ⊆ E2 -> wp SI E1 e Φ -∗ (∀ v, Φ v ={E2}=∗ Ψ v) -∗ wp SI E2 e Ψ.
-Proof.
-  iIntros (Hmask).
-  iLöb as "IH" forall (e).
-  rewrite wp_unfold.
-  rewrite wp_unfold.
-  iIntros "Hwp H".
-  destruct e; simpl.
-  - 
-   iDestruct ("H" with "Hwp") as "H". 
-   iDestruct (fupd_mask_mono _ _ _ Hmask with "H") as "H'".
-   repeat (iMod "H'").
-   done. 
-  - 
-    iMod (fupd_mask_subseteq E1) as "Hclose"; first done. 
-    iMod "Hwp". iIntros "!> !>". 
-    iMod "Hwp". iMod "Hclose".
-    iModIntro.
-    iApply ("IH" $! e with "Hwp H").
-  - 
-    iMod (fupd_mask_subseteq E1) as "Hclose"; first done. 
-    iMod "Hwp". iIntros "!> !>".
-    iMod "Hwp" as "(Hwpe2 & $)".
-    iMod "Hclose".
-    iModIntro.
-    iApply ("IH" $! e2 with "Hwpe2 H").
-  - iIntros (σ) "HSi".
-    iMod (fupd_mask_subseteq E1) as "Hclose"; first done. 
-    iMod ("Hwp" with "HSi") as "Hwp".
-    iIntros "!> !>".
-    iMod "Hwp". iMod "Hclose". iModIntro.
-    iDestruct "Hwp" as (σ' v) "(Hcom & HSi & Hwp)".
-    iExists σ', v. iFrame. 
-    iApply ("IH"  with "Hwp H"). 
-Qed.
-
-Lemma wp_strong_mono_bupd {V R: Type} (SI: gmap nat V -> iProp Σ) (E: coPset)
-  (e: expr V R) (Φ Ψ: R -> iProp Σ)
-  : wp SI E e Φ -∗ (∀ v, Φ v ==∗ Ψ v) -∗ wp SI E e Ψ.
-Proof.
-  iIntros "Hwp Hf".
-  iApply (wp_strong_mono_fupd with "Hwp"); first set_solver.
-  - iIntros (v) "Hphi".
-    iMod ("Hf" with "Hphi") as "Hf".
-    iModIntro. done.
-Qed.
-
-Lemma wp_mono' {V R: Type} (SI: gmap nat V -> iProp Σ) (E: coPset)
-   (e: expr V R) (Φ Ψ: R -> iProp Σ)
-   : (∀ v, Φ v -∗ Ψ v) -> wp SI E e Φ -∗  wp SI E e Ψ.
-Proof.
-  iIntros (Hv) "Hwp".
-  iApply (wp_strong_mono_fupd with "Hwp"); first set_solver.
-  - iIntros (v) "Hphi". 
-    iModIntro.
-    iApply (Hv with "Hphi").
-Qed.
-
-Lemma wp_mono {V R: Type} (SI: gmap nat V -> iProp Σ) (E: coPset)
-   (e: expr V R) (Φ Ψ: R -> iProp Σ)
-   :wp SI E e Φ -∗ (∀ v, Φ v -∗ Ψ v) -∗ wp SI E e Ψ.
-Proof.
-  iIntros "Hwp H".
-  iApply (wp_strong_mono_fupd with "Hwp"); first set_solver.
-  - iIntros (v) "Hphi". 
-    iModIntro.
-    iApply ("H" with "Hphi").
-Qed.
-
-Lemma wp_fmap {V R B: Type} (SI: gmap nat V -> iProp Σ) (E: coPset)
-  (f: R -> B) (Φ: B -> iProp Σ) (e: expr V R)
-  : wp SI E e (Φ ∘ f ) -∗ wp SI E (f <$> e) Φ. 
-Proof.
-  iIntros "Hwp".
-  iApply wp_bind.
-  iApply (wp_mono with "Hwp").
-  iIntros (x) "Hpost /=".
-  iApply (wp_return with "Hpost").
-Qed.
-
-Lemma wp_iter {V R B: Type} (SI: gmap nat V -> iProp Σ) (E: coPset) (Φ: B -> iProp Σ)
-  (x: R)
-  (f: R -> expr V (R + B)):
-  wp SI E (f x) (case_ (λ x, ▷ wp SI E (iter f x) Φ) Φ) -∗
-  wp SI E (iter f x) Φ.
-Proof.
-  iIntros "Hwp".
-  rewrite iter_unfold.
-  iApply wp_bind.
-  iApply (wp_mono with "Hwp").
-  iIntros ([a | b]) "H /=".
-  - by iApply wp_think.
-  - by iApply wp_return.
-Qed.
-
-Lemma fupd_wp {V R: Type} (SI: gmap nat V -> iProp Σ) (E: coPset)
- (e: expr V R) (Φ : R -> iProp Σ)
- : (|={E}=> wp SI E e Φ) ⊢ wp SI E e Φ.
-Proof.
-  iIntros "Hwp".
-  rewrite wp_unfold.
-  unfold wp_pre.
-  destruct e.
-  - iMod "Hwp" as "Hwp".
-    by iMod "Hwp" as "Hwp".
-  - iMod "Hwp" as "Hwp".
-    by iMod "Hwp" as "Hwp".
-  - iMod "Hwp" as "Hwp".
-    by iMod "Hwp" as "Hwp".
-  - by iMod "Hwp" as "Hwp".
-Qed.
-
-Lemma bupd_wp {V R: Type} (SI: gmap nat V -> iProp Σ) (E: coPset)
- (e: expr V R) (Φ : R -> iProp Σ)
- : (|==> wp SI E e Φ) ⊢ wp SI E e Φ.
-Proof.
-  iIntros "Hwp".
-  rewrite wp_unfold.
-  unfold wp_pre.
-  destruct e.
-  - iMod "Hwp" as "Hwp".
-    by iMod "Hwp" as "Hwp".
-  - iMod "Hwp" as "Hwp".
-    by iMod "Hwp" as "Hwp".
-  - iMod "Hwp" as "Hwp".
-    by iMod "Hwp" as "Hwp".
-  - by iMod "Hwp" as "Hwp".
-Qed.
-
-Lemma wp_fupd {V R: Type} (SI: gmap nat V -> iProp Σ) (E: coPset)
- (e: expr V R) (Φ : R -> iProp Σ) 
- : wp SI E e (λ v, |={E}=> Φ v) ⊢ wp SI E e Φ.
-Proof.
-  iIntros "Hwp".
-  iApply (wp_strong_mono_fupd with "Hwp"); first set_solver.
-  auto.
-Qed.
-
-Lemma wp_bupd {V R: Type} (SI: gmap nat V -> iProp Σ) (E: coPset)
- (e: expr V R) (Φ : R -> iProp Σ) 
- : wp SI E e (λ v, |==> Φ v) ⊢ wp SI E e Φ.
-Proof.
-  iIntros "Hwp".
-  iApply (wp_strong_mono_bupd with "Hwp").
-  auto.
-Qed.
-
-Lemma wp_think' {V R: Type} (SI: gmap nat V -> iProp Σ) (E: coPset) 
-  (e: expr V R) (Φ: R -> iProp Σ)
-  : wp SI E (Think e) Φ ={E, ∅}=∗ ▷ |={∅, E}=> wp SI E e Φ .
-Proof.
-  iIntros "Hwp".
-  rewrite wp_unfold. 
-  unfold wp_pre.
-  done.
-Qed.
-
-Lemma wp_frame_r {V R: Type} (SI: gmap nat V -> iProp Σ) (E: coPset) 
-  (e: expr V R) (Φ: R -> iProp Σ) (P: iProp Σ)
-  : ((wp SI E e Φ) ∗ P) ⊢ wp SI E e (λ v, Φ v ∗ P).
+  Instance wp_pre_contractive {A SI}: Contractive (@wp_pre A SI).
   Proof.
-    iIntros "[Hwp Hp]".
-    iApply (wp_strong_mono_bupd with "Hwp").
-    auto with iFrame.
+    rewrite /wp_pre => n wp wp' Hwp R E e1 Φ.
+    repeat (f_contractive || f_equiv); apply Hwp.
   Qed.
 
-Lemma wp_frame_l {V R: Type} (SI: gmap nat V -> iProp Σ) (E: coPset) 
-  (e: expr V R) (Φ: R -> iProp Σ) (P: iProp Σ)
-  : (P ∗ (wp SI E e Φ) ) ⊢ wp SI E e (λ v, P ∗ Φ v ).
+  Definition wp' {V} (SI: gmap nat V -> iProp Σ):
+    ∀R, coPset -> expr V R -> (R -> iProp Σ) ->iProp Σ :=
+      fixpoint (wp_pre SI).
+
+  Definition wp {V R} (SI: gmap nat V -> iProp Σ) (E: coPset) (e: expr V R) (Φ: R -> iProp Σ): iProp Σ := 
+      wp' SI R E e Φ.
+
+  Definition wp_thread {V R} (SI: gmap nat V -> iProp Σ) (t: thread V R):
+    (R -> iProp Σ) -> iProp Σ :=
+      match t with
+      | Main e => wp SI ⊤ e
+      | Forked e => λ _,  wp SI ⊤ e (λ _, True%I)
+      end.
+
+  Lemma wp'_unfold {V R} (SI: gmap nat V -> iProp Σ) 
+    (E: coPset) (e: expr V R) (Φ: R -> iProp Σ):
+      wp' SI R E e Φ  ≡  wp_pre SI (wp' SI) R E e Φ.
   Proof.
-    iIntros "[Hp Hwp]".
-    iApply (wp_strong_mono_bupd with "Hwp").
-    auto with iFrame.
+    apply (fixpoint_unfold (wp_pre SI)).
   Qed.
 
-  Lemma wp_fork {V: Type} (SI: gmap nat V -> iProp Σ) (e: expr V ()) (E: coPset) (Φ: () -> iProp Σ):
-   ▷ wp SI ⊤ e (λ _, True) -∗ Φ () -∗ wp SI E (itree.fork e) Φ.
+  Lemma wp_unfold {V R} (SI: gmap nat V -> iProp Σ)
+    (E: coPset) (e: expr V R) (Φ: R -> iProp Σ):
+      wp SI E e Φ  ≡  wp_pre SI (wp' SI) R E e Φ.
   Proof.
-    iIntros "Hwpf HΦ".
-    iEval( rewrite wp_unfold). unfold wp_pre.
+    apply (fixpoint_unfold (wp_pre SI)).
+  Qed.
+
+  Lemma wp_return {V R: Type} (SI: gmap nat V -> iProp Σ) (E: coPset)
+     (x: R) (Φ: R -> iProp Σ): Φ x -∗ wp SI E (mret x) Φ.
+  Proof.
+    iIntros"H".
+    by rewrite wp_unfold.
+  Qed.
+
+  Lemma wp_think {V R: Type} (SI: gmap nat V -> iProp Σ) (E: coPset)
+    (e: expr V R) (Φ: R -> iProp Σ):
+      ▷ wp SI E e Φ -∗ wp SI E (Think e) Φ.
+  Proof.
+    iIntros "Hwp".
+    iEval (rewrite wp_unfold).
+    unfold wp_pre.
     iApply fupd_mask_intro; first set_solver.
-    iIntros "Hclose !>". iMod "Hclose". iModIntro.
-    iFrame. by iApply wp_return.
+    iIntros "H".
+    iNext. iMod "H". iModIntro.
+    done.
   Qed.
+
+  Lemma wp_bind {V R B: Type} (SI: gmap nat V -> iProp Σ) (E: coPset)
+    (f: R -> expr V B) (Φ: B -> iProp Σ) (e: expr V R):
+      wp SI E e (λ x, wp SI E (f x) Φ) -∗ wp SI E (e ≫= f) Φ.
+  Proof.
+    unfold mbind, itree_bind.
+    iIntros "H". iLöb as "IH" forall (e).
+    iEval (rewrite wp_unfold).
+    unfold wp_pre.
+    destruct e; simpl.
+    - do 2 (rewrite wp_unfold /=). unfold wp_pre.
+      by destruct (f r); iMod "H".
+    - iEval (rewrite wp_unfold /=) in "H".
+      iMod "H". iIntros "!> !>". iApply "IH". done.
+    - iEval (rewrite wp_unfold /=) in "H".
+      iMod "H". iIntros "!> !>". iMod "H" as "(H & $)".
+      iApply "IH". done.
+    - iIntros (σ)  "HSi".
+      iEval (rewrite wp_unfold /=) in "H".
+      iMod ("H" $! σ with "HSi") as "H". iModIntro.
+      iNext.
+      iMod ("H") as (σ' v) "H". iModIntro.
+      iExists σ', v.
+      iDestruct "H" as "($ & $ & Hwp)".
+      iApply "IH". done.
+  Qed.
+
+  Lemma wp_vup {V R: Type} (SI: gmap nat V -> iProp Σ) (E: coPset)
+    (e: expr V R) (Φ: R -> iProp Σ):
+      (|={E}=> wp SI E e (λ v, |={E}=> Φ v)) ⊢ wp SI E e Φ.
+  Proof.
+    iLöb as "IH" forall (e).
+    iIntros "Hwp".
+    rewrite wp_unfold. rewrite wp_unfold.
+    unfold wp_pre.
+    destruct e; simpl.
+    - repeat (iMod "Hwp"). done.
+    - iMod "Hwp". 
+      iMod "Hwp". iModIntro.
+      iNext. 
+      iMod "Hwp". iModIntro.
+      iApply "IH". done.
+    - repeat (iMod "Hwp").
+      iModIntro. iNext.
+      iMod "Hwp" as "(Hwp & $)".
+      iApply "IH". done.
+    - iIntros (σ) "HSi".
+      iMod "Hwp".
+      iDestruct ("Hwp" with "HSi" ) as "Hwp".
+      iMod "Hwp". iModIntro. iNext.
+      iMod "Hwp". iModIntro.
+      iDestruct ("Hwp") as (σ' v) "(Hcmd & HSi & Hwp)".
+      iExists σ', v. iFrame.
+      iApply "IH". done.
+  Qed.
+
+  Variant atomic {V R: Type}: expr V R -> Prop :=
+  |answer_atomic:  ∀x, atomic (Answer x)
+  |think_atomic:   ∀x, atomic (Think (Answer x))
+  |vis_atomic:     ∀c, atomic (Vis c Answer).
+
+  Lemma wp_atomic {V R: Type} (SI: gmap nat V -> iProp Σ) (E1 E2: coPset)
+    (e: expr V R) (Φ: R -> iProp Σ) (a: atomic e):
+      (|={E1, E2}=> wp SI E2 e (λ v, |={E2, E1}=> Φ v)) ⊢ wp SI E1 e Φ.
+  Proof.
+    iIntros "Hwp".
+    rewrite wp_unfold. 
+    rewrite wp_unfold. 
+    destruct a; simpl.
+    - iMod "Hwp". iMod "Hwp". iMod "Hwp".
+      done.
+    - iMod "Hwp". iMod "Hwp". iModIntro.
+      iNext. iMod "Hwp". 
+      rewrite wp'_unfold. rewrite wp'_unfold. simpl.
+      iMod "Hwp".  iMod "Hwp". done.
+    - iIntros (σ) "HSi".
+      iMod "Hwp". iDestruct ("Hwp" with "HSi") as "Hwp".
+      iMod "Hwp". iModIntro. iNext. iMod "Hwp".
+      iDestruct ("Hwp") as (σ' v) "(Hcmd & HSi & Hwp)".
+      iExists σ', v. iFrame.
+      rewrite wp'_unfold. rewrite wp'_unfold. simpl.
+      iMod "Hwp". iMod "Hwp".
+      done.
+  Qed.
+
+  Lemma wp_strong_mono_fupd {V R: Type} (SI: gmap nat V -> iProp Σ) (E1 E2: coPset)
+    (e: expr V R) (Φ Ψ: R -> iProp Σ):
+      E1 ⊆ E2 -> wp SI E1 e Φ -∗ (∀ v, Φ v ={E2}=∗ Ψ v) -∗ wp SI E2 e Ψ.
+  Proof.
+    iIntros (Hmask).
+    iLöb as "IH" forall (e).
+    rewrite wp_unfold.
+    rewrite wp_unfold.
+    iIntros "Hwp H".
+    destruct e; simpl.
+    - 
+     iDestruct ("H" with "Hwp") as "H". 
+     iDestruct (fupd_mask_mono _ _ _ Hmask with "H") as "H'".
+     repeat (iMod "H'").
+     done. 
+    - 
+      iMod (fupd_mask_subseteq E1) as "Hclose"; first done. 
+      iMod "Hwp". iIntros "!> !>". 
+      iMod "Hwp". iMod "Hclose".
+      iModIntro.
+      iApply ("IH" $! e with "Hwp H").
+    - 
+      iMod (fupd_mask_subseteq E1) as "Hclose"; first done. 
+      iMod "Hwp". iIntros "!> !>".
+      iMod "Hwp" as "(Hwpe2 & $)".
+      iMod "Hclose".
+      iModIntro.
+      iApply ("IH" $! e2 with "Hwpe2 H").
+    - iIntros (σ) "HSi".
+      iMod (fupd_mask_subseteq E1) as "Hclose"; first done. 
+      iMod ("Hwp" with "HSi") as "Hwp".
+      iIntros "!> !>".
+      iMod "Hwp". iMod "Hclose". iModIntro.
+      iDestruct "Hwp" as (σ' v) "(Hcom & HSi & Hwp)".
+      iExists σ', v. iFrame. 
+      iApply ("IH"  with "Hwp H"). 
+  Qed.
+
+  Lemma wp_strong_mono_bupd {V R: Type} (SI: gmap nat V -> iProp Σ) (E: coPset)
+    (e: expr V R) (Φ Ψ: R -> iProp Σ):
+      wp SI E e Φ -∗ (∀ v, Φ v ==∗ Ψ v) -∗ wp SI E e Ψ.
+  Proof.
+    iIntros "Hwp Hf".
+    iApply (wp_strong_mono_fupd with "Hwp"); first set_solver.
+    - iIntros (v) "Hphi".
+      iMod ("Hf" with "Hphi") as "Hf".
+      iModIntro. done.
+  Qed.
+
+  Lemma wp_mono' {V R: Type} (SI: gmap nat V -> iProp Σ) (E: coPset)
+    (e: expr V R) (Φ Ψ: R -> iProp Σ):
+      (∀ v, Φ v -∗ Ψ v) -> wp SI E e Φ -∗  wp SI E e Ψ.
+  Proof.
+    iIntros (Hv) "Hwp".
+    iApply (wp_strong_mono_fupd with "Hwp"); first set_solver.
+    - iIntros (v) "Hphi". 
+      iModIntro.
+      iApply (Hv with "Hphi").
+  Qed.
+
+  Lemma wp_mono {V R: Type} (SI: gmap nat V -> iProp Σ) (E: coPset)
+    (e: expr V R) (Φ Ψ: R -> iProp Σ):
+      wp SI E e Φ -∗ (∀ v, Φ v -∗ Ψ v) -∗ wp SI E e Ψ.
+  Proof.
+    iIntros "Hwp H".
+    iApply (wp_strong_mono_fupd with "Hwp"); first set_solver.
+    - iIntros (v) "Hphi". 
+      iModIntro.
+      iApply ("H" with "Hphi").
+  Qed.
+
+  Lemma wp_fmap {V R B: Type} (SI: gmap nat V -> iProp Σ) (E: coPset)
+    (f: R -> B) (Φ: B -> iProp Σ) (e: expr V R):
+      wp SI E e (Φ ∘ f ) -∗ wp SI E (f <$> e) Φ. 
+  Proof.
+    iIntros "Hwp".
+    iApply wp_bind.
+    iApply (wp_mono with "Hwp").
+    iIntros (x) "Hpost /=".
+    iApply (wp_return with "Hpost").
+  Qed.
+
+  Lemma wp_iter {V R B: Type} (SI: gmap nat V -> iProp Σ) (E: coPset) (Φ: B -> iProp Σ)
+    (x: R) (f: R -> expr V (R + B)):
+      wp SI E (f x) (case_ (λ x, ▷ wp SI E (iter f x) Φ) Φ) 
+      -∗ wp SI E (iter f x) Φ.
+  Proof.
+    iIntros "Hwp".
+    rewrite iter_unfold.
+    iApply wp_bind.
+    iApply (wp_mono with "Hwp").
+    iIntros ([a | b]) "H /=".
+    - by iApply wp_think.
+    - by iApply wp_return.
+  Qed.
+
+  Lemma fupd_wp {V R: Type} (SI: gmap nat V -> iProp Σ) (E: coPset)
+   (e: expr V R) (Φ : R -> iProp Σ):
+    (|={E}=> wp SI E e Φ) ⊢ wp SI E e Φ.
+  Proof.
+    iIntros "Hwp".
+    rewrite wp_unfold.
+    unfold wp_pre.
+    destruct e.
+    - iMod "Hwp" as "Hwp".
+      by iMod "Hwp" as "Hwp".
+    - iMod "Hwp" as "Hwp".
+      by iMod "Hwp" as "Hwp".
+    - iMod "Hwp" as "Hwp".
+      by iMod "Hwp" as "Hwp".
+    - by iMod "Hwp" as "Hwp".
+  Qed.
+
+  Lemma bupd_wp {V R: Type} (SI: gmap nat V -> iProp Σ) (E: coPset)
+   (e: expr V R) (Φ : R -> iProp Σ):
+     (|==> wp SI E e Φ) ⊢ wp SI E e Φ.
+  Proof.
+    iIntros "Hwp".
+    rewrite wp_unfold.
+    unfold wp_pre.
+    destruct e.
+    - iMod "Hwp" as "Hwp".
+      by iMod "Hwp" as "Hwp".
+    - iMod "Hwp" as "Hwp".
+      by iMod "Hwp" as "Hwp".
+    - iMod "Hwp" as "Hwp".
+      by iMod "Hwp" as "Hwp".
+    - by iMod "Hwp" as "Hwp".
+  Qed.
+
+  Lemma wp_fupd {V R: Type} (SI: gmap nat V -> iProp Σ) (E: coPset)
+   (e: expr V R) (Φ : R -> iProp Σ):
+      wp SI E e (λ v, |={E}=> Φ v) ⊢ wp SI E e Φ.
+  Proof.
+    iIntros "Hwp".
+    iApply (wp_strong_mono_fupd with "Hwp"); first set_solver.
+    auto.
+  Qed.
+
+  Lemma wp_bupd {V R: Type} (SI: gmap nat V -> iProp Σ) (E: coPset)
+   (e: expr V R) (Φ : R -> iProp Σ):
+      wp SI E e (λ v, |==> Φ v) ⊢ wp SI E e Φ.
+  Proof.
+    iIntros "Hwp".
+    iApply (wp_strong_mono_bupd with "Hwp").
+    auto.
+  Qed.
+
+  Lemma wp_think' {V R: Type} (SI: gmap nat V -> iProp Σ) (E: coPset) 
+    (e: expr V R) (Φ: R -> iProp Σ):
+      wp SI E (Think e) Φ ={E, ∅}=∗ ▷ |={∅, E}=> wp SI E e Φ .
+  Proof.
+    iIntros "Hwp".
+    rewrite wp_unfold. 
+    unfold wp_pre.
+    done.
+  Qed.
+
+  Lemma wp_frame_r {V R: Type} (SI: gmap nat V -> iProp Σ) (E: coPset) 
+    (e: expr V R) (Φ: R -> iProp Σ) (P: iProp Σ):
+      ((wp SI E e Φ) ∗ P) ⊢ wp SI E e (λ v, Φ v ∗ P).
+    Proof.
+      iIntros "[Hwp Hp]".
+      iApply (wp_strong_mono_bupd with "Hwp").
+      auto with iFrame.
+    Qed.
+
+  Lemma wp_frame_l {V R: Type} (SI: gmap nat V -> iProp Σ) (E: coPset) 
+    (e: expr V R) (Φ: R -> iProp Σ) (P: iProp Σ):
+      (P ∗ (wp SI E e Φ) ) ⊢ wp SI E e (λ v, P ∗ Φ v ).
+    Proof.
+      iIntros "[Hp Hwp]".
+      iApply (wp_strong_mono_bupd with "Hwp").
+      auto with iFrame.
+    Qed.
+
+    Lemma wp_fork {V: Type} (SI: gmap nat V -> iProp Σ) (e: expr V ()) (E: coPset) (Φ: () -> iProp Σ):
+      ▷ wp SI ⊤ e (λ _, True) -∗ Φ () -∗ wp SI E (itree.fork e) Φ.
+    Proof.
+      iIntros "Hwpf HΦ".
+      iEval( rewrite wp_unfold). unfold wp_pre.
+      iApply fupd_mask_intro; first set_solver.
+      iIntros "Hclose !>". iMod "Hclose". iModIntro.
+      iFrame. by iApply wp_return.
+    Qed.
 End itreewp.
 
 Section heap_wp.
@@ -372,7 +362,7 @@ Section heap_wp.
   Context `{!invGS Σ}.
   Context (γ: gname).
 
-  Lemma wp_get n v E (Ψ: V -> iProp Σ) :
+  Lemma wp_get n v E (Ψ: V -> iProp Σ):
     points_to γ n v -∗ (points_to γ n v -∗ Ψ v) -∗ wp (state_interp γ) E (itree.get n) Ψ.
   Proof.
     iIntros "Hpt Hpost".
@@ -386,8 +376,8 @@ Section heap_wp.
     iApply wp_return. by iApply "Hpost".
   Qed.
 
-  Lemma wp_get' n v E (Ψ: V -> iProp Σ) :
-   ▷ points_to γ n v -∗ ▷ (points_to γ n v -∗ Ψ v) -∗ wp (state_interp γ) E (itree.get n) Ψ.
+  Lemma wp_get' n v E (Ψ: V -> iProp Σ):
+    ▷ points_to γ n v -∗ ▷ (points_to γ n v -∗ Ψ v) -∗ wp (state_interp γ) E (itree.get n) Ψ.
   Proof.
     iIntros "Hpt Hpost".
     rewrite wp_unfold. unfold wp_pre.
@@ -400,7 +390,7 @@ Section heap_wp.
     iApply wp_return. by iApply "Hpost".
   Qed.
 
-  Lemma wp_put n v v' E (Ψ: unit -> iProp Σ) :
+  Lemma wp_put n v v' E (Ψ: unit -> iProp Σ): 
     points_to γ n v -∗ (points_to γ n v' -∗ Ψ tt) -∗ wp (state_interp γ) E (itree.put n v') Ψ.
   Proof.
     iIntros "Hpt Hpost".
@@ -419,7 +409,7 @@ Section heap_wp.
       by iApply "Hpost".
   Qed. 
 
-  Lemma wp_put' n v v' E (Ψ: unit -> iProp Σ) :
+  Lemma wp_put' n v v' E (Ψ: unit -> iProp Σ):
     ▷ points_to γ n v -∗ ▷ (points_to γ n v' -∗ Ψ tt) -∗ wp (state_interp γ) E (itree.put n v') Ψ.
   Proof.
     iIntros "Hpt Hpost".
@@ -477,7 +467,7 @@ Section heap_wp.
   Qed.
 
   Lemma wp_free' v l E (Ψ: unit -> iProp Σ):
-   ▷ points_to γ l v -∗ Ψ tt -∗ wp (state_interp γ) E (itree.free l) Ψ.
+    ▷ points_to γ l v -∗ Ψ tt -∗ wp (state_interp γ) E (itree.free l) Ψ.
   Proof.
     iIntros "Hpt Hpost". 
     rewrite wp_unfold. unfold wp_pre.
@@ -576,8 +566,6 @@ Section heap_wp.
       iApply wp_return.
       by iApply "HPost".
   Qed.
-
-
 End heap_wp.
 
 
@@ -595,8 +583,7 @@ Section proofmode_classes.
   Global Instance frame_wp p E e R Φ Ψ :
     (∀ v, Frame p R (Φ v) (Ψ v)) →
     Frame p R (wp SI E e Φ) (wp SI E e Ψ) | 2.
-  Proof. rewrite /Frame=> HR. rewrite wp_frame_l. apply wp_mono', HR.
-  Qed.
+  Proof. rewrite /Frame=> HR. rewrite wp_frame_l. apply wp_mono', HR. Qed.
 
   Global Instance is_except_0_wp E e Φ : IsExcept0 (wp SI E e Φ).
   Proof. by rewrite /IsExcept0 -{2}fupd_wp -except_0_fupd -fupd_intro. Qed.
@@ -657,33 +644,23 @@ Section adequacy.
   Context `{!invGS Σ}. 
 
   (*
-    Ok what does this bugger say again?
-
-    We are stepping in e.
-    With two post conditions ψ is the post condition for the expression
-    we are stepping right now.
-    Φ is the post condition for the main thread, thus it is the one that matters
-    for the rest of the threadpool. Since forked threads discard it, it only applies
-    to the main thread.
-
-    Since this is the deepest level it seems we should use the soundness lemmas at this point.
-    Except no. We do not take in account that Φ and Ψ are pure. They are any iProp predicates.
-    Hence none of the soundness lemma's apply here.
+    We are taking a step in expression e.
+    With two post conditions ψ is the post condition for the expression e.
+    Φ is the post condition for the main thread, thus it is the one that matters for the rest of the threadpool. 
+    Since forked threads discard it, it only applies to the main thread.
   *)
   Lemma step_expr_adequacy {R A} {cmp: EqDecision V} (γ: gname) (Φ: R -> iProp Σ) (Ψ: A -> iProp Σ)
-    (h: heap V)
-    (ts: list (thread V R))
-    (e: expr V A)
-    : wp (state_interp γ) ⊤ e Ψ
-    -∗ state_interp γ h
-    ={⊤, ∅}=∗ 
-     ▷ |={∅, ⊤}=> match runState (step_expr e) h ts with
-       | Here (e', h', ts') => ∃ts'', ⌜ts' = ts ++ ts''⌝ 
-                               ∗ wp (state_interp γ) ⊤ e' Ψ ∗ state_interp γ h'
-                               ∗ [∗ list] t ∈ ts'', wp_thread (state_interp γ) t Φ
-       | ProgErr => False
-       | EvalErr => True
-       end.
+    (h: heap V) (ts: list (thread V R)) (e: expr V A):
+      wp (state_interp γ) ⊤ e Ψ
+      -∗ state_interp γ h
+      ={⊤, ∅}=∗ ▷ |={∅, ⊤}=>
+        match runState (step_expr e) h ts with
+          | Here (e', h', ts') => ∃ts'', ⌜ts' = ts ++ ts''⌝ 
+                     ∗ wp (state_interp γ) ⊤ e' Ψ ∗ state_interp γ h'
+                     ∗ [∗ list] t ∈ ts'', wp_thread (state_interp γ) t Φ
+          | ProgErr => False
+          | EvalErr => True
+          end.
   Proof.
     iIntros "Hwp Hsi".
     destruct e; simpl.
@@ -744,27 +721,24 @@ Section adequacy.
 
   (* 
    We still have two post conditions, but they operate on the same type now.
-   Ψ is for the thread we are stepping. Ah so this is the above lifted to a thread.
+   Ψ is for the thread we are stepping. So this is the above lifted to a thread.
    Φ is still the post condition for the main thread.
   *)
   Lemma step_thread_adequacy {R} {cmp: EqDecision V} (γ: gname) (Φ Ψ: R -> iProp Σ)
-    (h: heap V)
-    (ts: list (thread V R))
-    (ct: thread V R)
-    : wp_thread (state_interp γ) ct Ψ 
-    -∗ state_interp γ h
-    ={⊤, ∅}=∗ 
-     ▷ |={∅, ⊤}=>
-      match runState (step_thread ct) h ts with
-      | Here (ct', h', ts') => ∃ts'', ⌜ts' = ts ++ ts''⌝
-                              ∗ wp_thread (state_interp γ) ct' Ψ ∗ state_interp γ h'
-                              ∗ [∗ list] t ∈ ts'', wp_thread (state_interp γ) t Φ
-      | ProgErr => False
-      | EvalErr => True
-      end.
+    (h: heap V) (ts: list (thread V R)) (ct: thread V R):
+      wp_thread (state_interp γ) ct Ψ 
+      -∗ state_interp γ h
+      ={⊤, ∅}=∗ ▷ |={∅, ⊤}=>
+        match runState (step_thread ct) h ts with
+        | Here (ct', h', ts') => ∃ts'', ⌜ts' = ts ++ ts''⌝
+                                ∗ wp_thread (state_interp γ) ct' Ψ ∗ state_interp γ h'
+                                ∗ [∗ list] t ∈ ts'', wp_thread (state_interp γ) t Φ
+        | ProgErr => False
+        | EvalErr => True
+        end.
   Proof.
     iIntros "Hwp Hsi".
-    simpl.
+    simpl. unfold step_thread.
     destruct ct; simpl.
     - 
       iMod (step_expr_adequacy _ _ _ _ ts  with "Hwp Hsi") as "Hexpr".
@@ -787,26 +761,24 @@ Section adequacy.
     by destruct l.
   Qed.
 
-  (*  OK third one up, now there is just one post condition left.
-      Φ for the main thread. All the other threads namely have the trivial
-      post condition
+  (*  
+    The next level incorparating the scheduler, now there is just one post condition left:
+    Φ for the main thread.
+    All the other threads namely have the trivial post condition
   *)
   Lemma scheduled_adequacy {R} {cmp: EqDecision V} (γ: gname) (Φ: R -> iProp Σ)
-    (h: heap V)
-    (s: scheduler V R)
-    (ts: list (thread V R))
-    : ts ≠ [] ->
-    state_interp γ h
-    -∗ ([∗ list] t ∈ ts, wp_thread (state_interp γ) t Φ)
-    ={⊤, ∅}=∗
-     ▷ |={∅, ⊤}=>
-      match runState (single_step_thread s) h ts with
-      | Here (s', h', ts') => ⌜length ts <= length ts'⌝
-                              ∗ state_interp γ h'
-                              ∗ [∗ list] t ∈ ts', wp_thread (state_interp γ) t Φ
-      | ProgErr => False
-      | EvalErr => True
-      end.
+    (h: heap V) (s: scheduler V R) (ts: list (thread V R)):
+      ts ≠ [] ->
+      state_interp γ h
+      -∗ ([∗ list] t ∈ ts, wp_thread (state_interp γ) t Φ)
+      ={⊤, ∅}=∗ ▷ |={∅, ⊤}=>
+        match runState (single_step_thread s) h ts with
+        | Here (s', h', ts') => ⌜length ts <= length ts'⌝
+                                ∗ state_interp γ h'
+                                ∗ [∗ list] t ∈ ts', wp_thread (state_interp γ) t Φ
+        | ProgErr => False
+        | EvalErr => True
+        end.
   Proof.
     iIntros (Hnil) "HSi Hbigop".
     unfold single_step_thread. simpl. destruct (schedule s (ts, h)) as [i s'].
@@ -829,14 +801,14 @@ Section adequacy.
 
   Arguments mbind_state : simpl never.
 
-  Lemma run_get_threads {A} σ (ts: list (thread V A))
-    : runState get_threads σ ts = Here (ts, σ, ts).
+  Lemma run_get_threads {A} σ (ts: list (thread V A)):
+    runState get_threads σ ts = Here (ts, σ, ts).
   Proof.
     done.
   Qed.
 
-  Lemma non_nil_bigger_than {A} {ts ts' : list A}
-    : ts ≠ [] -> length ts ≤ length ts' -> ts' ≠ [].
+  Lemma non_nil_bigger_than {A} {ts ts' : list A}:
+    ts ≠ [] -> length ts ≤ length ts' -> ts' ≠ [].
   Proof.
     intros Hnil Hlength.
     destruct ts'.
@@ -849,7 +821,8 @@ Section adequacy.
   Qed.
 
   (*
-    I need the conclusion to say something about how ts can be split up
+    When the first thread is checked to be the first thread,
+    then the whole list of threads can be split up between the Main thread and a tail.
   *)
   Lemma check_main_head {A: Type} (ts: list (thread V A)) (r: A)
     : check_main ts = Some r -> ∃ts', ts = (Main $ Answer r) :: ts'.
@@ -866,38 +839,32 @@ Section adequacy.
           subst r. done.
         + done.
     Qed.
-  (* 
-    Get the iterated update lemma's into their own file,
-    iApply nlaters to introduce them
-    Then use the eqn from check_main to prove that:
-    the first entry in ts' is a Main.
-    That that thread is a Here.
-    Then get the post condition out.
 
-    The modalities seem to misallign here, it looks like
-    it should be iterating |==> ▷ |==>?
-    is that legal? Yes, Yes it is.
+  (*
+    The adequacy lemma with the recursive knot tied by the fuel evaluator.
+    We build on top of scheduled_adequacy and induction on the fuel.
+    We need to iterate the modality pattern of: |==> ▷ |==>.
+    Since that many updates or steps might be required if the entire amount of fuel is used
+    by the evaluator.
+    If they are not required by the computation we can introduce them using fupd_nlaters.
   *)
   Lemma fuel_adequacy {R} {cmp: EqDecision V} (γ: gname) (Φ: R -> iProp Σ) (n: nat)
-    (h: heap V)
-    (s: scheduler V R)
-    (ts: list (thread V R))
-    : ts ≠ [] -> 
-    state_interp γ h
-    -∗ ([∗ list] t ∈ ts, wp_thread (state_interp γ) t Φ) 
-    -∗ Nat.iter n (λ P : iPropI Σ, |={⊤, ∅}=> ▷ |={∅,⊤}=> P) 
-        match runState (eval_threaded n s) h ts with
-        | Here (x, h', ts') => Φ x 
-        | ProgErr => False
-        | EvalErr => True
-        end.
+    (h: heap V) (s: scheduler V R) (ts: list (thread V R)):
+      ts ≠ [] 
+      -> state_interp γ h
+      -∗ ([∗ list] t ∈ ts, wp_thread (state_interp γ) t Φ) 
+      -∗ Nat.iter n (λ P : iPropI Σ, |={⊤, ∅}=> ▷ |={∅,⊤}=> P) 
+           match runState (eval_threaded n s) h ts with
+           | Here (x, h', ts') => Φ x 
+           | ProgErr => False
+           | EvalErr => True
+           end.
   Proof.
     iInduction n as [|n'] "IH" forall (s h ts);
     iIntros (Hnil) "Hsi Hbigop".
     - done.
     - iPoseProof (scheduled_adequacy _ _ _ s  with "Hsi Hbigop" ) as "H"; try done.
-      iEval (unfold eval_threaded). fold (eval_threaded (V := nat) (R := R)).
-      rewrite run_bind_dist.
+      iEval (unfold eval_threaded). rewrite run_bind_dist.
       destruct (runState (single_step_thread _)  h ts) as [[[s' σ'] ts'] | | ]; try done.
       +
         rewrite run_bind_dist.
@@ -921,41 +888,30 @@ Section adequacy.
       + iSimpl. iMod "H". iIntros "!> !>". iMod "H". iModIntro.
         iApply fupd_nlaters; first set_solver. done.
   Qed.
-
 End adequacy.
 
 
 (*
   So what needs to happen here?
-  1. I need to be in an iris context to use fuel_adequacy
+  1. We need to be in an iris context to use fuel_adequacy
      because it uses wands rather than coq arrows.
   2. To be able to lift the entailment from hpre like in adequacy_state_delay
-     I will need to get a gname to allocate the initial heap.
-     Why is there a gname in my context already? ok that was from the section,
-     it is removed now.
-  3. How do I get a gname? that is from this snippet:
-    but that requires a bupd at the top level.
-    can I change the soundness lemma to give me that?
+     We will need to get a gname to allocate the initial heap.
+  3. How do we get a gname? that is from this snippet:
      iMod (own_alloc (● (lift_excl st))) as (γ) "Hsi".
-  4. When should I call lift entailment?
-  5. Atleast I have my initial bupd from the soundness lemma now.
-  6. I want to call fuel_adequacy, for that I need a big op of
-     wp's for all threads. That list is [Main e]. However
-     I have a wp for e in Hpre as expr not a thread.
-     let's lift that.
-     Now I need to get it in a big op
+     but that requires a bupd at the top level therefore we require
+     n + 1 modalities. From step_fupdN_soundness'
+  4. Then we can call fuel_adequacy.
 *)
 Lemma adequacy {V Σ} {cmp: EqDecision V} `{!inG Σ (heapR V)} `{!invGpreS Σ} {R}
-  (φ: R -> Prop) (n: nat)
-  (SI: gmap nat V -> iProp Σ)
-  (s: scheduler V R)
-  (e: expr V R)
-  : (∀ `{!invGS Σ} γ, ⊢ wp (state_interp γ) ⊤ e (λ x, ⌜φ x⌝)) ->
-  match run_program n s e with
-  | Here x => φ x
-  | ProgErr => False
-  | EvalErr => True
-  end.
+  (φ: R -> Prop) (n: nat) (SI: gmap nat V -> iProp Σ)
+  (s: scheduler V R) (e: expr V R):
+    (∀ `{!invGS Σ} γ, ⊢ wp (state_interp γ) ⊤ e (λ x, ⌜φ x⌝)) ->
+      match run_program n s e with
+      | Here x => φ x
+      | ProgErr => False
+      | EvalErr => True
+      end.
   Proof.
     intros Hpre.
     unfold run_program.
